C2_Sims_filter.v
@@ -1,0 +1,1 @@
+(* A functional Sims-filter to reduce generator sets. *)
