C3_generator_chain.v
@@ -1,0 +1,1 @@
+(* The Scheier-Sims algorithm to factor a group into a chain of subgroups. *)
